Add parse function in `core.str`

CoqOfRust/core/str.v
@@ -1,8 +1,87 @@
 Require Import CoqOfRust.lib.lib.
 
+Require CoqOfRust.core.result.
+
 Module error.
   Module ParseBoolError.
     Parameter t : Set.
   End ParseBoolError.
   Definition ParseBoolError := ParseBoolError.t.
 End error.
+
+Module FromStr.
+  Class Trait (Self : Set) : Type := { 
+    Err : Set;
+    from_str :
+      ref str.t ->
+      M (result.Result.t Self Err);
+  }.
+End FromStr.
+
+Module FromStr_instances.
+  #[refine]
+  Global Instance for_bool : FromStr.Trait bool := {
+    Err := str.error.ParseBoolError;
+  }.
+    all: destruct (axiom "FromStr_instances" : Empty_set).
+  Defined.
+
+  Global Instance for_char : FromStr.Trait char.t.
+  Admitted.
+
+  Global Instance for_f32 : FromStr.Trait f32.t.
+  Admitted.
+
+  Global Instance for_f64 : FromStr.Trait f64.t.
+  Admitted.
+
+  Global Instance for_i8 : FromStr.Trait i8.t.
+  Admitted.
+
+  Global Instance for_i16 : FromStr.Trait i16.t.
+  Admitted.
+
+  Global Instance for_i32 : FromStr.Trait i32.t.
+  Admitted.
+
+  Global Instance for_i64 : FromStr.Trait i64.t.
+  Admitted.
+
+  Global Instance for_i128 : FromStr.Trait i128.t.
+  Admitted.
+
+  Global Instance for_isize : FromStr.Trait isize.t.
+  Admitted.
+
+  Global Instance for_u8 : FromStr.Trait u8.t.
+  Admitted.
+
+  Global Instance for_u16 : FromStr.Trait u16.t.
+  Admitted.
+
+  Global Instance for_u32 : FromStr.Trait u32.t.
+  Admitted.
+
+  Global Instance for_u64 : FromStr.Trait u64.t.
+  Admitted.
+
+  Global Instance for_u128 : FromStr.Trait u128.t.
+  Admitted.
+
+  Global Instance for_usize : FromStr.Trait usize.t.
+  Admitted.
+End FromStr_instances.
+
+Module Impl_str.
+  Definition Self : Set := str.t.
+
+  Parameter parse :
+    forall {F : Set} {H0 : FromStr.Trait F},
+    ref Self ->
+    M (core.result.Result.t F (FromStr.Err (Trait := H0))).
+
+  Global Instance AssociatedFunction_parse {F : Set} {H0 : FromStr.Trait F} :
+    Notations.DoubleColon Self "parse" := {
+    Notations.double_colon := parse (F := F);
+  }.
+End Impl_str.
